SystemFD/Algorithm/Soundness2.lean
@@ -1,0 +1,509 @@
+import SystemFD.Term
+import SystemFD.Judgment
+import SystemFD.Ctx
+import SystemFD.Algorithm
+import SystemFD.Algorithm.Soundness1
+
+theorem infer_type_sound : infer_type Γ t = .some A -> ⊢ Γ -> Γ ⊢ t : A := by
+intro h wf
+induction Γ, t using infer_type.induct generalizing A <;> simp at *
+case _ ih =>
+  rw [Option.bind_eq_some] at h
+  cases h; case _ u1 h =>
+  cases h; case _ h1 h2 =>
+    replace h1 := wf_kind_sound h1 wf
+    constructor; apply h1
+    apply ih h2; constructor
+    apply h1; apply wf
+case _ ih =>
+  rw [Option.bind_eq_some] at h
+  cases h; case _ u1 h =>
+  cases h; case _ h1 h2 =>
+  rw [Option.bind_eq_some] at h2
+  cases h2; case _ u2 h2 =>
+  cases h2; case _ h2 h3 =>
+  rw [Option.bind_eq_some] at h3
+  cases h3; case _ u3 h3 =>
+  cases h3; case _ h3 h4 =>
+  simp at h4; cases h4; case _ h4 h5 =>
+    subst h5; replace h2 := is_pointed_some h2; subst h2
+    have lem := infer_kind_sound h1 wf
+    constructor; apply lem; apply h4
+    apply ih h3; constructor; apply lem; apply wf
+    apply h4
+case _ ih =>
+  rw [Option.bind_eq_some] at h
+  cases h; case _ u1 h =>
+  cases h; case _ h1 h2 =>
+    have lem := wf_kind_sound h1 wf
+    constructor; apply lem
+    apply ih h2; constructor
+    apply lem; apply wf
+case _ ih =>
+  rw [Option.bind_eq_some] at h
+  cases h; case _ u1 h =>
+  cases h; case _ h1 h2 =>
+  rw [Option.bind_eq_some] at h2
+  cases h2; case _ u2 h2 =>
+  cases h2; case _ h2 h3 =>
+    replace h2 := is_const_some h2; subst h2
+    replace h1 := infer_kind_sound h1 wf
+    constructor; apply h1; apply ih h3
+    constructor; apply h1; apply wf
+case _ ih =>
+  rw [Option.bind_eq_some] at h
+  cases h; case _ u1 h =>
+  cases h; case _ h1 h2 =>
+  rw [Option.bind_eq_some] at h2
+  cases h2; case _ u2 h2 =>
+  cases h2; case _ h2 h3 =>
+    replace h2 := is_const_some h2; subst h2
+    replace h1 := infer_kind_sound h1 wf
+    constructor; apply h1; apply ih h3
+    constructor; apply h1; apply wf
+case _ ih1 ih2 =>
+  rw [Option.bind_eq_some] at h
+  cases h; case _ u1 h =>
+  cases h; case _ h1 h2 =>
+  rw [Option.bind_eq_some] at h2
+  cases h2; case _ u2 h2 =>
+  cases h2; case _ h2 h3 =>
+  rw [Option.bind_eq_some] at h3
+  cases h3; case _ u3 h3 =>
+  cases h3; case _ h3 h4 =>
+  simp at h4; cases h4; case _ h4 h5 =>
+    replace h4 := Term.eq_of_beq h4; subst h4; subst h5
+    replace h1 := is_openm_some h1
+    constructor; rw [h1]; apply ih1 h2 wf
+    apply ih2 h3; constructor; rw [h1]
+    apply ih1 h2 wf; apply wf
+case _ ih1 ih2 =>
+  rw [Option.bind_eq_some] at h
+  cases h; case _ u1 h =>
+  cases h; case _ h1 h2 =>
+  rw [Option.bind_eq_some] at h2
+  cases h2; case _ u2 h2 =>
+  cases h2; case _ h2 h3 =>
+  rw [Option.bind_eq_some] at h3
+  cases h3; case _ u3 h3 =>
+  cases h3; case _ h3 h4 =>
+  rw [Option.bind_eq_some] at h4
+  cases h4; case _ u4 h4 =>
+  cases h4; case _ h4 h5 =>
+  simp at h5; cases h5; case _ h5 h6 =>
+    replace h5 := Term.eq_of_beq h5; subst h5; subst h6
+    replace h2 := is_const_some h2; subst h2
+    replace h1 := infer_kind_sound h1 wf
+    constructor; apply h1; apply ih1 h3 wf
+    apply ih2 h4; constructor; apply h1
+    apply ih1 h3 wf; apply wf
+case _ => constructor; apply wf; rw [h]
+case _ Γ p s i e ih1 ih2 ih3 ih4 =>
+  rw [Option.bind_eq_some] at h
+  cases h; case _ u1 h =>
+  cases h; case _ h1 h2 =>
+  rw [Option.bind_eq_some] at h2
+  cases h2; case _ u2 h2 =>
+  cases h2; case _ h2 h3 =>
+  rw [Option.bind_eq_some] at h3
+  cases h3; case _ u3 h3 =>
+  cases h3; case _ h3 h4 =>
+  rw [Option.bind_eq_some] at h4
+  cases h4; case _ u4 h4 =>
+  cases h4; case _ h4 h5 =>
+  rw [Option.bind_eq_some] at h5
+  cases h5; case _ u5 h5 =>
+  cases h5; case _ h5 h6 =>
+  rw [Option.bind_eq_some] at h6
+  cases h6; case _ u6 h6 =>
+  cases h6; case _ h6 h7 =>
+  rw [Option.bind_eq_some] at h7
+  cases h7; case _ u7 h7 =>
+  cases h7; case _ h7 h8 =>
+  rw [Option.bind_eq_some] at h8
+  cases h8; case _ u8 h8 =>
+  cases h8; case _ h8 h9 =>
+  generalize zdef :
+    infer_kind Γ ([P' (List.length u1.to_telescope.fst)]Term.from_telescope_rev u8.reverse u7.to_telescope.snd) = z
+    at h9
+  rw [Option.bind_eq_some] at h9
+  cases h9; case _ u9 h9 =>
+  cases h9; case _ h9 h10 =>
+  rw [Option.bind_eq_some] at h10
+  cases h10; case _ u10 h10 =>
+  cases h10; case _ h10 h11 =>
+  rw [Option.bind_eq_some] at h11
+  cases h11; case _ u11 h11 =>
+  cases h11; case _ h11 h12 =>
+  simp at h12; cases h12; case _ h12 h13 =>
+  cases h12; case _ h12 h14 =>
+  cases h12; case _ h12 h15 =>
+    sorry
+case _ Γ p s t ih1 ih2 ih3 =>
+  rw [Option.bind_eq_some] at h
+  cases h; case _ u1 h =>
+  cases h; case _ h1 h2 =>
+  rw [Option.bind_eq_some] at h2
+  cases h2; case _ u2 h2 =>
+  cases h2; case _ h2 h3 =>
+  rw [Option.bind_eq_some] at h3
+  cases h3; case _ u3 h3 =>
+  cases h3; case _ h3 h4 =>
+  rw [Option.bind_eq_some] at h4
+  cases h4; case _ u4 h4 =>
+  cases h4; case _ h4 h5 =>
+  rw [Option.bind_eq_some] at h5
+  cases h5; case _ u5 h5 =>
+  cases h5; case _ h5 h6 =>
+  rw [Option.bind_eq_some] at h6
+  cases h6; case _ ξ h6 =>
+  cases h6; case _ h6 h7 =>
+  rw [Option.bind_eq_some] at h7
+  cases h7; case _ u7 h7 =>
+  cases h7; case _ h7 h8 =>
+  rw [Option.bind_eq_some] at h8
+  cases h8; case _ u8 h8 =>
+  cases h8; case _ h8 h9 =>
+  simp at h9; cases h9; case _ h9 h10 =>
+  cases h9; case _ h9 h11 =>
+  cases h9; case _ h9 h12 =>
+    replace h3 := is_unpointed_some h3; subst h3
+    replace h8 := is_const_some h8; subst h8; subst h10
+    replace h9 := Term.eq_of_beq h9; subst h9
+    replace h2 := infer_kind_sound h2 wf
+    replace h7 := infer_kind_sound h7 wf
+    replace h1 := ih1 h1 wf
+    replace h4 := ih2 h4 wf
+    replace h5 := ih3 h5 wf
+    replace h11 := Term.eq_of_beq h11
+    replace h12 := Term.eq_of_beq h12
+    generalize τdef : u1.to_telescope.fst = τ at *
+    generalize sRdef : u1.to_telescope.snd = sR at *
+    have lem1 : (τ, sR) = u1.to_telescope := by sorry
+    generalize τpdef : u5.to_telescope.fst = τ' at *
+    generalize sTdef : u5.to_telescope.snd = sT at *
+    have lem3 : (τ', sT) = u5.to_telescope := by sorry
+    apply @Judgment.guard Γ p u1 τ sR ([P' (List.length τ)]sR) s t u5 τ' sT ξ (Term.from_telescope ξ sT) _ _
+    apply h1; apply lem1; simp; apply h12; apply h2; apply h4; apply h5
+    apply lem3; rw [h6]; rfl; simp; apply h11; apply h7
+case _ ih =>
+  rw [Option.bind_eq_some] at h
+  cases h; case _ u1 h =>
+  cases h; case _ h1 h2 =>
+  rw [Option.bind_eq_some] at h2
+  cases h2; case _ u2 h2 =>
+  cases h2; case _ h2 h3 =>
+  rw [Option.bind_eq_some] at h3
+  cases h3; case _ u3 h3 =>
+  cases h3; case _ h3 h4 =>
+    injection h4 with e; subst e
+    replace h2 := is_const_some h2; subst h2
+    replace h1 := infer_kind_sound h1 wf
+    constructor; apply h1; apply ih h3
+    constructor; apply h1; apply wf
+case _ ih1 ih2 =>
+  rw [Option.bind_eq_some] at h
+  cases h; case _ u1 h =>
+  cases h; case _ h1 h2 =>
+  rw [Option.bind_eq_some] at h2
+  cases h2; case _ u2 h2 =>
+  cases h2; case _ h2 h3 =>
+  rw [Option.bind_eq_some] at h3
+  cases h3; case _ u3 h3 =>
+  cases h3; case _ h3 h4 =>
+  simp at h4; cases h4; case _ h4 h5 =>
+    replace h2 := is_arrow_some h2; subst h2
+    replace h4 := Term.eq_of_beq h4; subst h4; subst h5
+    constructor; apply ih1 h1 wf
+    apply ih2 h3 wf; rfl
+case _ ih =>
+  rw [Option.bind_eq_some] at h
+  cases h; case _ u1 h =>
+  cases h; case _ h1 h2 =>
+  rw [Option.bind_eq_some] at h2
+  cases h2; case _ u2 h2 =>
+  cases h2; case _ h2 h3 =>
+    replace h1 := wf_kind_sound h1 wf
+    injection h3 with e; subst e
+    constructor; apply h1; apply ih h2
+    constructor; apply h1; apply wf
+case _ ih =>
+  rw [Option.bind_eq_some] at h
+  cases h; case _ u1 h =>
+  cases h; case _ h1 h2 =>
+  rw [Option.bind_eq_some] at h2
+  cases h2; case _ u2 h2 =>
+  cases h2; case _ h2 h3 =>
+  rw [Option.bind_eq_some] at h3
+  cases h3; case _ u3 h3 =>
+  cases h3; case _ h3 h4 =>
+  simp at h4; cases h4; case _ h4 h5 =>
+    replace h4 := Term.eq_of_beq h4; subst h4; subst h5
+    replace h2 := is_all_some h2; subst h2
+    replace h3 := infer_kind_sound h3 wf
+    constructor; apply ih h1 wf; apply h3; rfl
+case _ ih1 ih2 =>
+  rw [Option.bind_eq_some] at h
+  cases h; case _ u1 h =>
+  cases h; case _ h1 h2 =>
+  rw [Option.bind_eq_some] at h2
+  cases h2; case _ u2 h2 =>
+  cases h2; case _ h2 h3 =>
+  rw [Option.bind_eq_some] at h3
+  cases h3; case _ u3 h3 =>
+  simp at h3; cases h3; case _ h3 h4 =>
+  cases h4; case _ h4 h5 =>
+    replace h4 := Term.eq_of_beq h4; subst h4; subst h5
+    replace h3 := is_eq_some h3; subst h3
+    constructor; apply ih1 h1 wf; apply ih2 h2 wf
+case _ =>
+  rw [Option.bind_eq_some] at h
+  cases h; case _ u1 h =>
+  cases h; case _ h1 h2 =>
+  rw [Option.bind_eq_some] at h2
+  cases h2; case _ u2 h2 =>
+  cases h2; case _ h2 h3 =>
+    replace h1 := infer_kind_sound h1 wf
+    replace h2 := is_pointed_some h2; subst h2
+    injection h3 with e; subst e
+    constructor; apply h1
+case _ ih =>
+  rw [Option.bind_eq_some] at h
+  cases h; case _ u1 h =>
+  cases h; case _ h1 h2 =>
+  rw [Option.bind_eq_some] at h2
+  cases h2; case _ h2 h3 =>
+  cases h3; case _ h3 h4 =>
+    injection h4 with e; subst e
+    replace h3 := is_eq_some h3; subst h3
+    constructor; apply ih h1 wf
+case _ ih1 ih2 =>
+  rw [Option.bind_eq_some] at h
+  cases h; case _ u1 h =>
+  rw [Option.bind_eq_some] at h
+  cases h; case _ h1 h2 =>
+  cases h2; case _ u2 h2 =>
+  cases h2; case _ h2 h3 =>
+  rw [Option.bind_eq_some] at h3
+  cases h3; case _ u3 h3 =>
+  cases h3; case _ h3 h4 =>
+  rw [Option.bind_eq_some] at h4
+  cases h4; case _ u4 h4 =>
+  cases h4; case _ h4 h5 =>
+  simp at h5; cases h5; case _ h5 h6 =>
+    replace h3 := is_eq_some h3; subst h3; subst h6
+    replace h4 := is_eq_some h4; subst h4
+    replace h5 := Term.eq_of_beq h5
+    constructor; apply ih1 h1 wf; rw [h5]
+    apply ih2 h2 wf
+case _ ih1 ih2 =>
+  rw [Option.bind_eq_some] at h
+  cases h; case _ u1 h =>
+  cases h; case _ h1 h2 =>
+  rw [Option.bind_eq_some] at h2
+  cases h2; case _ u2 h2 =>
+  cases h2; case _ h2 h3 =>
+  rw [Option.bind_eq_some] at h3
+  cases h3; case _ u3 h3 =>
+  cases h3; case _ h3 h4 =>
+  rw [Option.bind_eq_some] at h4
+  cases h4; case _ u4 h4 =>
+  cases h4; case _ h4 h5 =>
+    injection h5 with e; subst e
+    replace h3 := is_eq_some h3; subst h3
+    replace h4 := is_eq_some h4; subst h4
+    constructor; apply ih1 h1 wf; apply ih2 h2 wf
+case _ ih1 ih2 =>
+  rw [Option.bind_eq_some] at h
+  cases h; case _ u1 h =>
+  cases h; case _ h1 h2 =>
+  rw [Option.bind_eq_some] at h2
+  cases h2; case _ u2 h2 =>
+  cases h2; case _ h2 h3 =>
+  rw [Option.bind_eq_some] at h3
+  cases h3; case _ u3 h3 =>
+  cases h3; case _ h3 h4 =>
+  rw [Option.bind_eq_some] at h4
+  cases h4; case _ u4 h4 =>
+  cases h4; case _ h4 h5 =>
+    injection h5 with e; subst e
+    replace h3 := is_eq_some h3; subst h3
+    replace h4 := is_eq_some h4; subst h4
+    replace h1 := ih1 h1 wf
+    constructor; apply h1; apply ih2 h2
+    constructor; apply wf
+case _ ih =>
+  rw [Option.bind_eq_some] at h
+  cases h; case _ u1 h =>
+  cases h; case _ h1 h2 =>
+  rw [Option.bind_eq_some] at h2
+  cases h2; case _ u2 h2 =>
+  cases h2; case _ h2 h3 =>
+  rw [Option.bind_eq_some] at h3
+  cases h3; case _ u3 h3 =>
+  cases h3; case _ h3 h4 =>
+  rw [Option.bind_eq_some] at h4
+  cases h4; case _ u4 h4 =>
+  cases h4; case _ h4 h5 =>
+    injection h5 with e; subst e
+    replace h2 := is_eq_some h2; subst h2
+    replace h3 := is_appk_some h3
+    replace h4 := is_appk_some h4
+    rw [h3, h4] at h1
+    constructor; apply ih h1 wf
+case _ ih =>
+  rw [Option.bind_eq_some] at h
+  cases h; case _ u1 h =>
+  cases h; case _ h1 h2 =>
+  rw [Option.bind_eq_some] at h2
+  cases h2; case _ u2 h2 =>
+  cases h2; case _ h2 h3 =>
+  rw [Option.bind_eq_some] at h3
+  cases h3; case _ u3 h3 =>
+  cases h3; case _ h3 h4 =>
+  rw [Option.bind_eq_some] at h4
+  cases h4; case _ u4 h4 =>
+  cases h4; case _ h4 h5 =>
+    injection h5 with e; subst e
+    replace h2 := is_eq_some h2; subst h2
+    replace h3 := is_appk_some h3
+    replace h4 := is_appk_some h4
+    rw [h3, h4] at h1
+    constructor; apply ih h1 wf
+case _ ih =>
+  rw [Option.bind_eq_some] at h
+  cases h; case _ u1 h =>
+  cases h; case _ h1 h2 =>
+  rw [Option.bind_eq_some] at h2
+  cases h2; case _ u2 h2 =>
+  cases h2; case _ h2 h3 =>
+  rw [Option.bind_eq_some] at h3
+  cases h3; case _ u3 h3 =>
+  cases h3; case _ h3 h4 =>
+    injection h4 with e; subst e
+    replace h3 := is_eq_some h3; subst h3
+    replace h1 := wf_kind_sound h1 wf
+    constructor; apply ih h2; constructor
+    apply h1; apply wf
+case _ ih1 ih2 =>
+  rw [Option.bind_eq_some] at h
+  cases h; case _ u1 h =>
+  cases h; case _ h1 h2 =>
+  rw [Option.bind_eq_some] at h2
+  cases h2; case _ u2 h2 =>
+  cases h2; case _ h2 h3 =>
+  rw [Option.bind_eq_some] at h3
+  cases h3; case _ u3 h3 =>
+  cases h3; case _ h3 h4 =>
+  rw [Option.bind_eq_some] at h4
+  cases h4; case _ u4 h4 =>
+  cases h4; case _ h4 h5 =>
+  rw [Option.bind_eq_some] at h5
+  cases h5; case _ u5 h5 =>
+  cases h5; case _ h5 h6 =>
+  rw [Option.bind_eq_some] at h6
+  cases h6; case _ u6 h6 =>
+  cases h6; case _ h6 h7 =>
+  simp at h7; cases h7; case _ h7 h8 =>
+    replace h7 := Term.eq_of_beq h7
+    replace h6 := is_eq_some h6; subst h6; subst h8
+    replace h3 := is_eq_some h3; subst h3
+    replace h4 := is_all_some h4
+    replace h5 := is_all_some h5
+    rw [h4] at h1; rw [h5] at h1; rw [h7] at h1
+    constructor; apply ih1 h1 wf; apply ih2 h2 wf
+
+theorem wf_ctx_sound : wf_ctx Γ = .some u -> ⊢ Γ := by
+intro h
+induction Γ using wf_ctx.induct generalizing u <;> simp at *
+case _ => constructor
+case _ ih => constructor; apply ih h
+case _ ih =>
+  rw [Option.bind_eq_some] at h
+  cases h; case _ u1 h =>
+  cases h; case _ h1 h2 =>
+  rw [Option.bind_eq_some] at h2
+  cases h2; case _ u2 h2 =>
+  cases h2; case _ h2 h3 =>
+    have lem := ih h3
+    replace h2 := is_const_some h2; subst h2
+    constructor; apply infer_kind_sound h1 lem; apply lem
+case _ ih =>
+  rw [Option.bind_eq_some] at h
+  cases h; case _ u1 h =>
+  cases h; case _ h1 h2 =>
+    have lem := ih h2
+    constructor; apply wf_kind_sound h1 lem; apply lem
+case _ ih =>
+  rw [Option.bind_eq_some] at h
+  cases h; case _ u1 h =>
+  cases h; case _ h1 h2 =>
+    have lem := ih h2
+    constructor; apply wf_kind_sound h1 lem; apply lem
+case _ ih =>
+  rw [Option.bind_eq_some] at h
+  cases h; case _ u1 h =>
+  cases h; case _ h1 h2 =>
+  rw [Option.bind_eq_some] at h2
+  cases h2; case _ u2 h2 =>
+  cases h2; case _ h2 h3 =>
+    simp at h3; have lem := ih h3.2
+    replace h2 := is_pointed_some h2; subst h2
+    constructor; apply infer_kind_sound h1 lem
+    apply lem; apply h3.1
+case _ ih =>
+  rw [Option.bind_eq_some] at h
+  cases h; case _ u1 h =>
+  cases h; case _ h1 h2 =>
+    have lem := ih h2
+    constructor; apply wf_kind_sound h1 lem; apply lem
+case _ ih =>
+  rw [Option.bind_eq_some] at h
+  cases h; case _ u1 h =>
+  cases h; case _ h1 h2 =>
+  rw [Option.bind_eq_some] at h2
+  cases h2; case _ u2 h2 =>
+  cases h2; case _ h2 h3 =>
+    have lem := ih h3
+    replace h2 := is_const_some h2; subst h2
+    constructor; apply infer_kind_sound h1 lem; apply lem
+case _ ih =>
+  rw [Option.bind_eq_some] at h
+  cases h; case _ u1 h =>
+  cases h; case _ h1 h2 =>
+  rw [Option.bind_eq_some] at h2
+  cases h2; case _ u2 h2 =>
+  cases h2; case _ h2 h3 =>
+    have lem := ih h3
+    replace h2 := is_const_some h2; subst h2
+    constructor; apply infer_kind_sound h1 lem; apply lem
+case _ ih =>
+  rw [Option.bind_eq_some] at h
+  cases h; case _ u1 h =>
+  cases h; case _ h1 h2 =>
+  rw [Option.bind_eq_some] at h2
+  cases h2; case _ u2 h2 =>
+  cases h2; case _ h2 h3 =>
+  rw [Option.bind_eq_some] at h3
+  cases h3; case _ u3 h3 =>
+  cases h3; case _ h3 h4 =>
+  rw [Option.bind_eq_some] at h4
+  cases h4; case _ u4 h4 =>
+  cases h4; case _ h4 h5 =>
+    simp at h5; replace h4 := ih h4
+    replace h5 := Term.eq_of_beq h5; subst h5
+    replace h2 := is_const_some h2; subst h2
+    constructor; apply infer_kind_sound h1 h4
+    apply infer_type_sound h3 h4; apply h4
+case _ hx ih =>
+  rw [hx] at h; simp at h
+  rw [Option.bind_eq_some] at h
+  cases h; case _ u1 h =>
+  cases h; case _ h1 h2 =>
+  rw [Option.bind_eq_some] at h2
+  cases h2; case _ u2 h2 =>
+  cases h2; case _ h2 h3 =>
+    simp at h3; replace h2 := ih h2
+    replace h3 := Term.eq_of_beq h3; subst h3
+    constructor; rw [hx]
+    apply infer_type_sound h1 h2; apply h2
