SystemFD/Metatheory/Classification.lean
@@ -1,0 +1,61 @@
+import SystemFD.Term
+import SystemFD.Term.Definition
+import SystemFD.Judgment
+import SystemFD.Ctx
+
+@[simp]
+abbrev class_idx (t A : Term) : JudgmentArgs v :=
+  match v with
+  | .prf => (t, A)
+  | .wf => ()
+
+@[simp]
+abbrev ClassType (Γ : Ctx Term) : (v : JudgmentVariant) -> JudgmentArgs v -> Prop
+| .prf => λ (_, A) => A = .kind ∨ (Γ ⊢ A : .kind) ∨ (∃ K, Γ ⊢ A : .const K)
+| .wf => λ () => ∀ x T, Frame.get_type (Γ d@ x) = .some T -> Γ ⊢ T : .kind ∨ (∃ K, Γ ⊢ T : .const K)
+
+theorem classification_lemma : Judgment v Γ ix -> ClassType Γ v ix := by
+intro j; induction j <;> simp at *
+all_goals (try simp [*])
+case _ => sorry
+case _ => sorry
+case _ => sorry
+case _ => sorry
+case _ => sorry
+case _ => sorry
+case _ => sorry
+case _ => sorry
+case _ => sorry
+case _ => sorry
+case _ => sorry
+case _ => sorry
+case _ => sorry
+case _ => sorry
+case _ => sorry
+case _ => sorry
+case _ => sorry
+case _ => sorry
+case _ j1 j2 ih1 ih2 =>
+  cases ih2
+  case _ ih2 =>
+    cases ih2; case _ ih2 =>
+      apply Or.inr; apply Or.inl; apply ih2
+  case _ ih2 =>
+  cases ih2; case _ K ih2 =>
+    cases ih2
+case _ j _ _ => apply Or.inl; constructor; apply judgment_ctx_wf j
+case _ => sorry
+case _ => sorry
+case _ => sorry
+case _ => sorry
+case _ => sorry
+case _ => sorry
+case _ => sorry
+case _ => sorry
+case _ => sorry
+case _ => sorry
+case _ => sorry
+case _ => sorry
+case _ => sorry
+case _ => sorry
+case _ => sorry
