SystemFD/Metatheory/Weaken.lean
@@ -1,0 +1,57 @@
+import SystemFD.Term
+import SystemFD.Judgment
+import SystemFD.Ctx
+
+-- theorem rename_lift r (A : Term) :
+--   (∀ x, [r.to](Γ d@ x) = Δ d@ (r x)) ->
+--   ∀ x, [r.lift.to]((A::Γ) d@ x) = ([r.to]A::Δ) d@ (Ren.lift r x)
+-- := by
+-- intro h x; simp
+-- cases x <;> simp at *
+-- case _ => rw [Subst.lift_lemma]; simp
+-- case _ x => rw [Subst.lift_lemma, <-h x]; simp
+
+@[simp]
+abbrev idx_ren (r : Ren) : JudgmentArgs v -> JudgmentArgs v :=
+  match v with
+  | .prf => λ (t, A) => ([r.to]t, [r.to]A)
+  | .wf => λ () => ()
+
+theorem rename (r : Ren) :
+  Judgment v Γ idx ->
+  ⊢ Δ ->
+  (∀ x, (Γ d@ x).apply r.to = Δ d@ (r x)) ->
+  Judgment v Δ (idx_ren r idx)
+:= by
+intro j wf h
+induction j <;> simp
+any_goals apply wf
+case _ Γ T t A j1 j2 ih1 ih2 => sorry
+case _ => sorry
+case _ => sorry
+case _ => sorry
+case _ => sorry
+case _ => sorry
+case _ => sorry
+case _ => sorry
+case _ => sorry
+case _ => sorry
+case _ => sorry
+case _ => sorry
+case _ => sorry
+case _ => sorry
+case _ => sorry
+case _ => sorry
+case _ => sorry
+case _ => sorry
+case _ => sorry
+case _ => sorry
+case _ => sorry
+case _ => sorry
+case _ => sorry
+case _ => sorry
+case _ => sorry
+case _ => sorry
+case _ => sorry
+case _ => sorry
+case _ => sorry
